checker/corresp.ml
@@ -5,22 +5,21 @@ module MT = MTypes
 module M = Model
 module H = Hashtbl
 module A = DynArray
+module C = Checker
 
 let lmap_of_model model =
   let lmap = H.create 3037 in
-  H.add lmap 254 (MT.Pos MT.CTrue) ;
-  M.lits_iteri (fun i _ lit -> H.add lmap (255+i) lit) model ;
+  M.lits_iteri (fun i _ lit -> H.add lmap (3+i) lit) model ;
   lmap
 
 let clause_table clauses =
   let ctable = H.create 11437 in
-  H.add ctable [MT.Pos MT.CTrue] () ;
-  List.iter (fun cl -> H.add ctable cl ()) clauses ;
+  List.iter (fun cl -> H.add ctable (List.sort compare cl) ()) clauses ;
   ctable
   
 let get_lit lmap k =
   try
-    H.find lmap k 
+    H.find lmap k
   with Not_found ->
     failwith
       (Format.sprintf "Unidentified literal identifier %d." k)
@@ -28,7 +27,11 @@ let get_lit lmap k =
 let tlit lmap = parser
   | [< 'GL.Kwd "-" ; 'GL.Int k >] ->
       MT.negate (get_lit lmap k)
-  | [< 'GL.Int k >] -> (get_lit lmap k)
+  | [< 'GL.Int k >] ->
+      if k < 0 then
+        MT.negate (get_lit lmap (-k))
+      else
+        get_lit lmap k
 
 
 let tclause lmap tokens =
@@ -48,7 +51,7 @@ let tentry lmap = parser
   | [< 'GL.Int id ; cl = tclause lmap ; ants = tantecedents >] ->
       (id, cl, ants)
 
-let check_clause model cltable clause =
+let check_clause model tauto_check cltable clause =
   begin
     if !COption.verbosity > 1
     then
@@ -57,10 +60,10 @@ let check_clause model cltable clause =
         (M.string_of_clause model clause)
   end ;
   try
-    let _ = H.find cltable clause in
+    let _ = H.find cltable (List.sort compare clause) in
     true
   with Not_found ->
-    if Builtins.tauto (M.get_bounds model) clause then
+    if tauto_check clause then
       true
     else
       begin
@@ -74,14 +77,44 @@ let check_clause model cltable clause =
         false
       end
 
-let check_entry model cltable (_, cl, ants) =
+let check_entry model tauto_check cltable (id, cl, ants) =
   match ants with
-  | [] -> check_clause model cltable cl
+  | [] ->
+      let okay = check_clause model tauto_check cltable cl in
+      if !COption.verbosity > 0 then
+        begin
+          if not okay then
+            let fmt = Format.err_formatter in
+            Format.fprintf fmt "Failed clause: %d@." id
+        end ;
+      okay
   | _ -> true
+
+let fallback model =
+  let bounds = M.get_bounds model in
+  let check_with checker cl =
+        let okay = checker.C.check bounds cl in
+        begin
+        if !COption.verbosity > 0 then
+          let fmt = Format.err_formatter in
+          Format.fprintf fmt "Fallback successful - %s@." checker.C.repr
+        end ;
+        okay
+      in
+  let all_checkers = M.get_all_checkers model in
+  fun cl ->
+      List.fold_left (fun b check -> b || check_with check cl)
+      (Builtins.tauto bounds cl) all_checkers
 
 let check model clauses tokens =
   let lmap = lmap_of_model model
   and ctable = clause_table clauses in
+  (* *)
+  let bounds = M.get_bounds model in
+  let tauto_check = Builtins.tauto bounds in
+  (*
+  let tauto_check = fallback model in
+  *)
   let rec check_aux tokens =
     match Stream.peek tokens with
     | None ->
@@ -90,6 +123,8 @@ let check model clauses tokens =
     | _ ->
       (* Get the next entry. *)
       let entry = tentry lmap tokens in
-      check_entry model ctable entry && check_aux tokens
+      (* check_entry model tauto_check ctable entry && check_aux tokens *)
+      let okay = check_entry model tauto_check ctable entry in
+      check_aux tokens && okay
   in
   check_aux tokens
