checker/coq/zset.v
@@ -1,69 +1,128 @@
 (* Module for integer sets. *)
 Require Import Bool.
 Require Import ZArith.
+Require MSets.
 Require Import prim.
 
-Definition zset : Type := list Z.
+Require Import Orders.
+Require Import Relations.
 
-Definition empty : zset := nil.
+Module Z_as_Int.
+  Open Scope Z_scope.
+  Definition t := Z.
+  Definition int := t.
+  Definition _0 := 0.
+  Definition _1 := 1.
+  Definition _2 := 2.
+  Definition _3 := 3.
+  Definition plus := Zplus.
+  Definition opp := Zopp.
+  Definition minus := Zminus.
+  Definition mult := Zmult.
+  Definition max := Zmax.
+  Definition gt_le_dec := Z_gt_le_dec.
+  Definition ge_lt_dec := Z_ge_lt_dec.
+  Definition eq_dec := Z_eq_dec.
+  Definition i2z : int -> Z := fun n => n.
+  Lemma i2z_eq : forall n p, i2z n=i2z p -> n = p.
+  Proof. intros; tauto. Qed.
+  Lemma i2z_0 : i2z _0 = 0.
+  Proof. intros; tauto. Qed.
+  Lemma i2z_1 : i2z _1 = 1.
+  Proof. intros; tauto. Qed.
+  Lemma i2z_2 : i2z _2 = 2.
+  Proof. intros; tauto. Qed.
+  Lemma i2z_3 : i2z _3 = 3.
+  Proof. intros; tauto. Qed.
+  Lemma i2z_plus : forall n p, i2z (n + p) = i2z n + i2z p.
+  Proof. intros; tauto. Qed.
+  Lemma i2z_opp : forall n, i2z (- n) = - i2z n.
+  Proof. intros; tauto. Qed.
+  Lemma i2z_minus : forall n p, i2z (n - p) = i2z n - i2z p.
+  Proof. intros; tauto. Qed.
+  Lemma i2z_mult : forall n p, i2z (n * p) = i2z n * i2z p.
+  Proof. intros; tauto. Qed.
+  Lemma i2z_max : forall n p, i2z (max n p) = Zmax (i2z n) (i2z p).
+  Proof. intros; tauto. Qed.
+End Z_as_Int.
 
-Fixpoint mem (s : zset) (k : Z) : Prop :=
-  match s with
-  | nil => False
-  | cons x xs => x = k \/ mem xs k
-  end.
+Module Z_as_OT <: OrderedType.
+  Definition t := Z.
+  Definition eq := @eq Z.
+  Definition eq_refl := @refl_equal t.
+  Definition eq_sym := @sym_eq t.
+  Definition eq_trans := @trans_eq t.
 
-Fixpoint memb (s : zset) (k : Z) : bool :=
-  match s with
-  | nil => false
-  | cons x xs => (Z_eqb x k) || memb xs k
-  end.
+  Program Instance eq_equiv : Equivalence eq.
 
-Theorem memb_true_iff_mem : forall (s : zset) (k : Z),
+  Definition lt (x y:Z) := (x<y).
+
+  Lemma lt_trans : forall x y z, x<y -> y<z -> x<z.
+  Proof. intros; omega. Qed.
+
+  Lemma lt_not_eq : forall x y, x<y -> ~ x=y.
+  Proof. intros; omega. Qed.
+
+  Definition compare := Zcompare.
+
+  Definition eq_dec := Z_eq_dec.
+
+  Program Instance lt_strorder : StrictOrder lt.
+  Program Definition lt_compat : Proper (eq ==> eq ==> iff) lt := _.
+  Lemma compare_spec : forall n m : Z, CompSpec eq lt n m (n ?= m).
+  Proof. apply Zcompare_spec. Qed.
+End Z_as_OT.
+
+Module ZSets := MSetAVL.IntMake(Z_as_Int)(Z_as_OT).
+
+Definition zset : Type := ZSets.t.
+
+Definition empty : zset := ZSets.empty.
+
+Definition mem (s : zset) (k : Z) : Prop := ZSets.In k s.
+Definition memb (s : zset) (k : Z) : bool := ZSets.mem k s.
+Definition memb_iff_mem : forall (s : zset) (k : Z),
   memb s k = true <-> mem s k.
 Proof.
-  intros. induction s.
   unfold memb, mem.
-  split. intros; discriminate.
-  intros; tauto.
-
-  unfold memb, mem; fold memb; fold mem.
-  rewrite <- Z_eqb_iff_eq. rewrite <- IHs.
-  rewrite orb_true_iff. tauto.
+  intros. apply ZSets.mem_spec.
 Qed.
 
-Definition add (s : zset) (k : Z) : zset :=
-  cons k s.
+Theorem notmem_empty : forall (k : Z),
+  ~ mem empty k.
+Proof.
+  unfold mem.
+  apply ZSets.empty_spec.
+Qed.
+
+Definition add (s : zset) (k : Z) : zset := ZSets.add k s.
 Theorem mem_mem_add : forall (s : zset) (k : Z) (k' : Z),
   mem s k -> mem (add s k') k.
 Proof.
-  intros; unfold add, mem. fold mem.
-  right. exact H.
+  unfold mem; intros. apply ZSets.add_spec.
+  right. assumption.
 Qed.
 Theorem mem_k_addk : forall (s : zset) (k : Z),
   mem (add s k) k.
 Proof.
-  intros; unfold add, mem; fold mem.
+  intros; unfold add, mem. rewrite ZSets.add_spec.
   left. trivial.
 Qed.
 Theorem mem_addk_if : forall (s : zset) (k k' : Z),
   mem (add s k) k' -> k = k' \/ mem s k'.
 Proof.
-  unfold add, mem; fold mem; intros.
-  exact H.
+  unfold add, mem;  intros.
+  apply ZSets.add_spec in H.
+  destruct H. eauto. eauto.
 Qed.
 
-Fixpoint rem (s : zset) (k : Z) :=
-  match s with
-  | nil => nil
-  | cons x xs =>
-    let tail := rem xs k in
-    if Z_eqb x k then tail else cons x tail
-  end.
+(*
+Fixpoint rem (s : zset) (k : Z) := ZSets.remove k s.
 Theorem notmem_k_remk : forall (s : zset) (k : Z),
   ~ mem (rem s k) k.
 Proof.
-  intros; induction s.
+  unfold mem, rem; intros.
+  apply ZSets.remove_spec.
 
   unfold mem, rem. tauto.
 
@@ -103,28 +162,182 @@ Proof.
   rewrite <- memb_true_iff_mem.
   tauto.
 Qed.
+*)
 
-Fixpoint union (xs ys : zset) :=
-  match xs with
-  | nil => ys
-  | cons x xs' => add (union xs' ys) x
-  end.
+Definition union (xs ys : zset) := ZSets.union xs ys.
 Theorem mem_union_iff : forall (xs ys : zset) (k : Z),
   mem (union xs ys) k <-> mem xs k \/ mem ys k.
 Proof.
-  induction xs.
-    unfold union.
-    split.
-      intro. right. exact H.
-    
-      unfold mem; fold mem. tauto.
+  unfold mem, union; apply ZSets.union_spec.
+Qed.
 
-    unfold union, mem; fold union; fold mem.
-    unfold add.
-    intros ys k.
-    assert (a = k \/ (mem xs k \/ mem ys k) <->
-      (a = k \/ mem xs k) \/ mem ys k). tauto.
-    rewrite <- H.
-    rewrite <- IHxs.
-    unfold mem; fold mem. tauto.
+Fixpoint zset_covers_nat (xs : zset) (k : Z) (sz : nat) :=
+  match sz with
+  | O => true
+  | S sz' => memb xs (k + (Z_of_nat sz')) && zset_covers_nat xs k sz'
+  end.
+Theorem zset_covers_nat_iff_covers :
+  forall (xs : zset) (k : Z) (sz : nat),
+    zset_covers_nat xs k sz = true <->
+      forall (sz' : nat), lt sz' sz -> mem xs (k + (Z_of_nat sz')).
+Proof.
+  intros xs k sz; induction sz.
+  unfold zset_covers_nat.
+  split.
+    intros; assert False. omega. tauto.
+    intros; trivial.
+
+  unfold zset_covers_nat; fold zset_covers_nat; rewrite andb_true_iff.
+  split.
+    intros; destruct H as [Hm Hc].
+    rewrite memb_iff_mem in Hm.
+    assert (lt sz' sz \/ sz' = sz) as Hle.
+      clear Hm Hc IHsz; omega.
+    destruct Hle as [Hle | Hle].
+    apply IHsz.
+      assumption. assumption.
+      rewrite Hle; assumption.
+
+  intros; rewrite memb_iff_mem.
+  split.
+    apply H; clear IHsz; omega.
+    apply IHsz.
+    intros; apply H. clear IHsz; omega.
+Qed.
+Definition zset_covers (xs : zset) (lb ub : Z) :=
+  if Z_leb lb ub then
+    zset_covers_nat xs lb (Zabs_nat (ub - lb + 1))
+  else
+    true.
+Theorem zset_covers_spec : forall (xs : zset) (lb ub : Z),
+  zset_covers xs lb ub = true <->
+    forall k, lb <= k <= ub -> mem xs k.
+Proof.
+  unfold zset_covers.
+  intros xs lb ub.
+  assert (Z_leb lb ub = true <-> lb <= ub).
+    apply Z_leb_iff_le.
+  destruct Z_leb.
+    assert (lb <= ub) as Hle. apply H; trivial. clear H.
+
+    split.
+      intros.
+      assert (k = (lb + (Z_of_nat (Zabs_nat (k - lb))))).
+      rewrite inj_Zabs_nat.
+      assert (k - lb >= 0).
+        omega.
+      rewrite Zabs_eq.
+        clear H. omega. omega.
+      rewrite zset_covers_nat_iff_covers in H.
+      rewrite H1.
+      apply H.
+      apply Zabs_nat_lt. omega.
+
+      intros. rewrite zset_covers_nat_iff_covers.
+      intros. apply H.
+      split. omega.
+      assert (ub = lb + Z_of_nat (Zabs_nat (ub - lb))).
+        rewrite inj_Zabs_nat. rewrite Zabs_eq.
+        omega.
+        omega.
+      rewrite H1. apply Zplus_le_compat.
+      omega. 
+      apply inj_le.
+      apply lt_n_Sm_le.
+      rewrite <- Zabs_nat_Zsucc.
+      assumption. omega.
+
+  assert (lb <= ub \/ ub < lb).
+    clear H; omega.
+  destruct H0.
+    apply H in H0; discriminate.
+  clear H.
+  split.
+    intros.
+      assert False. omega. tauto.
+    intros; trivial.
+Qed.
+
+Definition zset_min_lb (xs : zset) (k : Z) :=
+  match ZSets.min_elt xs with
+  | None => k
+  | Some k' => Zmin k k'
+  end.
+Theorem zset_min_lb_le : forall (xs : zset) (k : Z),
+  zset_min_lb xs k <= k.
+Proof.
+  unfold zset_min_lb.
+  intros xs k.
+  destruct ZSets.min_elt.
+    apply Zle_min_l.
+    omega.
+Qed.
+
+Theorem lt_min_notin_zset : forall (xs :zset) (k k' : Z),
+  k' < zset_min_lb xs k -> ~ mem xs k'.
+Proof.
+  unfold zset_min_lb; intros xs k k'.
+  assert (ZSets.min_elt xs = None -> ZSets.Empty xs).
+    apply ZSets.min_elt_spec3.
+  assert (forall m, ZSets.min_elt xs = Some m -> (forall n, mem xs n -> ~ n < m)).
+    unfold mem.
+    intros.
+    apply ZSets.min_elt_spec2 with (y := n) in H0.
+    assumption. assumption.
+  intros.
+  assert (~mem xs k' \/ mem xs k'). tauto.
+  destruct H2. assumption.
+  induction ZSets.min_elt.
+  apply Z.min_glb_lt_iff in H1.
+  destruct H1.
+  assert (~ k' < a).
+    apply H0. trivial. assumption.
+  omega.
+  
+  assert (ZSets.Empty xs).
+    apply H; trivial.
+  unfold ZSets.Empty in H3.
+  unfold mem. apply H3.
+Qed.
+
+Definition zset_max_ub (xs : zset) (k : Z) :=
+  match ZSets.max_elt xs with
+  | None => k
+  | Some k' => Zmax k k'
+  end.
+Theorem zset_max_ub_lb : forall (xs : zset) (k : Z),
+  k <= zset_max_ub xs k.
+Proof.
+  unfold zset_max_ub.
+  intros xs k.
+  destruct ZSets.max_elt.
+    apply Zle_max_l.
+    omega.
+Qed.
+
+Theorem max_lt_notin_zset : forall (xs :zset) (k k' : Z),
+  zset_max_ub xs k < k' -> ~ mem xs k'.
+Proof.
+  unfold zset_max_ub; intros xs k k'.
+  assert (ZSets.max_elt xs = None -> ZSets.Empty xs).
+    apply ZSets.max_elt_spec3.
+  assert (forall m, ZSets.max_elt xs = Some m -> (forall n, mem xs n -> ~ m < n)).
+    unfold mem.
+    intros.
+    apply ZSets.max_elt_spec2 with (y := n) in H0.
+    assumption. assumption.
+  intros.
+  assert (~mem xs k' \/ mem xs k'). tauto.
+  destruct H2. assumption.
+  induction ZSets.max_elt.
+  apply Z.max_lub_lt_iff in H1.
+  destruct H1.
+  assert (~ a < k').
+    apply H0. trivial. assumption.
+  omega.
+  
+  assert (ZSets.Empty xs).
+    apply H; trivial.
+  unfold ZSets.Empty in H3.
+  unfold mem. apply H3.
 Qed.
