checker/coq/checker_impl.v
@@ -11,14 +11,17 @@ Require element.
 Set Extraction Optimize.
 Extraction "checker_impl.ml"
   prim.check_inf prim.check_clause
-  bounds.check_tauto
-  bounds.check_tauto_bnd
+  (* domain.check_tauto *)
+  domain.check_tauto_bnd
+  (*
   cumulative.check_cumul
   cumulative.check_cumul_tt
+  *)
   cumulative.check_cumul_bnd
+  cumulative.check_cumul_tt_bnd
   reif.check_reif
-  linear.check_lincon
+  (* linear.check_lincon *)
   linear.check_linear_bnd
-  element.check_element
+  (* element.check_element *)
   element.check_element_bnd
   nat_of_int int_of_nat.
